pulse/ulib/experimental/Steel.Loops.fst
@@ -1,0 +1,40 @@
+module Steel.Loops
+open Steel.Memory
+open Steel.Effect.Common
+open Steel.Effect
+open Steel.Reference
+module AT = Steel.Effect.Atomic
+module U32 = FStar.UInt32
+
+val for_loop' (start:U32.t)
+              (finish:U32.t { U32.v start <= U32.v finish })
+              (current:U32.t { U32.v start <= U32.v current /\
+                               U32.v current <= U32.v finish })
+              (inv: nat_at_most finish -> vprop)
+              (body:
+                    (i:u32_between start finish ->
+                          SteelT unit
+                          (inv (U32.v i))
+                          (fun _ -> inv (U32.v i + 1))))
+  : SteelT unit
+      (inv (U32.v current))
+      (fun _ -> inv (U32.v finish))
+
+#push-options "--fuel 0 --ifuel 0"
+let rec for_loop' start finish current inv body
+  = if current = finish then (
+       AT.change_equal_slprop (inv _) (inv _);
+       AT.return ()
+    )
+    else (
+      let _: squash (U32.v current < U32.v finish) = () in //fails without this
+      body current;
+      let current' = U32.(current +^ 1ul) in
+      AT.change_equal_slprop (inv (U32.v current + 1))
+                             (inv (U32.v current'));
+      for_loop' start finish current' inv body
+    )
+
+
+(* produces 11 queries *)
+let for_loop start finish inv body = for_loop' start finish start inv body
